lemma chap1-HL: qed.

exercise-files/chap1-HL.ec
@@ -3,10 +3,9 @@ pragma Goals: printall.
 require import AllCore.
 
 (*
-Let us start small and work with some examples that we saw in the text.
-Please pay attention to the syntax of the modules,
-and capitalization of some names.
-EC expects the first letters of module names,
+Let us start small and first work with some examples that we saw in the text.
+Please pay attention to the syntax of the modules, and capitalization of names.
+EasyCrypt (EC) expects the first letters of module names,
 and module type names to be capitalized.
 *)
 
@@ -26,19 +25,19 @@ module Func1 = {
 EC allows us to define concretely defined procedures like we did above.
 But since we want to model adversaries about whom we know nothing,
 we can also define abstract procedures like an eavesdrop procedure 
-of an evil adversary. We don't know what the procedure does, but we
-do know its return type. We will return to this later when we
-start working with cryptographic protocols. But this is
-an important fact that we need to keep in mind.
-
-Also notice that now we have a module type and not just a module.
-This is because, Evil_adv is a type that we will need to instantiate.
-
+of an evil adversary. Like so:
 *)
-
 module type Evil_adv = {
   proc eavesdrop () : bool
 }.
+
+(*
+We don't know what the procedure does, but we do know its return type.
+Also notice that now we have a module type and not just a module.
+This is because, Evil_adv is a type that we will need to instantiate.
+We will return to this later when we start working with cryptographic protocols.
+But this is an important fact that we need to keep in mind.
+*)
 
 (* 
 Let us return to hoare triples and take a look at some triples and
@@ -69,7 +68,6 @@ is the ambient logic formula P => Q,
 where P is the original conclusion’s precondition, 
 and Q is its postcondition.
 *)
-
 skip.
 
 (*
@@ -82,8 +80,8 @@ a different name spaces to deal with them.
 To introduce memory into the context we need to prepend "&" to a variable name.
 Like so:
 *)
-
 move => &m H1.
+
 subst.
 (* The "subst" tactic simply substitutes variables *)
 trivial.
@@ -93,26 +91,44 @@ qed.
 lemma triple2: hoare [ Func1.add_2 : x = 1 ==> res = 3 ].
 proof.
 proc.
+
 (*
-
 Now we have a program which is not empty,
-so we can't use the skip tactic directly. 
-Thankfully we learnt about postcondition weakening.
-Take a look at this proof-tree. Applying the "wp" tactic
-computes the weakest precondition that needs to hold by
-consuming program statements and replacing the conclusion's
-postcondition with the weakest precondition R such that the 
-statement judgement consisting of R, the consumed suffix(es) and
-the conclusion’s original postcondition holds.
+so we can't use the "skip" tactic directly.
+Thankfully we learnt about the different axioms in hoare logic.
 
-                {x = 1} x:= x+2 {x=3}
-          -------------------------------wp
-                 {x = 1}     {x+2=3}
-          -------------------------------skip
-                   x = 1  => x+2=3
+When we are faced with 
+{P} S1; S2; S3; {Q}
+where P, and Q are pre and post conditions as usual,
+and S1; S2; S3 are statments of a program.
 
-  (* TODO: Show it formally once (help) *)
+Applying the "wp" tactic consumes as many ordinary statements as possible from
+the end. Then it replaces the postcondition Q, with the weakest precondition R.
+R is such that R in conjunction with the consumed statements and the original 
+post condition hold. It is easier to see as a visualization.
+
+            {P} S1; S2; S3 {Q}
+  --------------------------------------wp
+       {P} S1; {R} /\ {R} S2; S3; {Q}
+  --------------------------------------
+               {P} S1; {R}
+
+The triple {R} S2; S3; {Q} is guaranteed to hold, and hence the goal transforms to
+just {P} S1; {R}
+
+In our context the proof tree looks like so.
+The wp tactic, consumes the only statement in the program.
+In this case an assignment, and replaces the variable like we'd expect.
+When we have an empty program, we can simply use the "skip" tactic
+and continue with our proof. 
+
+             {x = 1} x:= x+2 {x=3}
+       -------------------------------wp
+              {x = 1}     {x+2=3}
+       -------------------------------skip
+                x = 1  => x+2=3
 *)
+
 wp.
 skip.
 move => &m x.
@@ -120,19 +136,32 @@ subst.
 trivial.
 qed.
 
-(* Using some automation *)
-
 (*
-We generally don't want to be dealing with the low-level proofs,
-so we will be combining Hoare logic with the automated tactics that
-we saw previously. One thing to remember is that the automated tactics
-work well with ambient logic.
+Let us define some more simple functions and hoare triples to work with.
 *)
 module Func2 = {
   proc x_sq (x:int) : int = { return x*x; }
   proc x_0  (x:int) : int = { x <- x*x; x<- x-x; return x; }
-  proc f_15 (x:int) : int = { x <- 15; return x; }
+  proc x_15 (x:int) : int = { x <- 15; return x; }
 }.
+
+(*
+Exercises:
+Define a few triples relating the behaviour of these functions.
+For instance try to define the following triples and prove them:
+1. {x = 2} Func2.x_sq {res = 4}
+2. {x= 10} Func2.x_0 {res = 0}
+3. {true} Func2.x_15 {res = 15}
+*)
+
+(* Using some automation *)
+
+(*
+We generally don't want to be dealing with the low-level proofs,
+so we will be combining Hoare logic with the external solvers that we saw earlier.
+One thing to remember is that the external solvers work only with ambient logic goals.
+So we need to get the goals state to something that the smt solvers can work with.
+*)
 
 lemma triple3: hoare [ Func2.x_sq : 4 <= x ==> 16 <= res ].
 proof.
@@ -174,7 +203,7 @@ However let us take a look at the next lemma. Now we are looking at the triple:
 This shouldn't hold, but watch what happens.
 *)
 
-lemma triple5: hoare [ Func2.f_15 : false ==> res=0 ].
+lemma triple5: hoare [ Func2.x_15 : false ==> res=0 ].
 proof.
 proc.
 wp.
@@ -193,47 +222,41 @@ to the assumptions.
 Pause here for a moment and ponder about what the goal currently says.
 It says that assuming that "false" holds, we want to prove that 15 = 0.
 As absurd as it is, we know that "false" is the strongest statement there is.
-And we have arrived to a state we say that "false" holds. This would imply that anything and
-everything can be derived from false. Hence we can actually "prove" that 15 = 0.
+And we have arrived to a state where "false" holds.
+This would imply that anything and everything can be derived from false.
+Hence we can actually "prove" that 15 = 0.
 *)
 trivial.
 qed.
 
 (*
 The point to understand here is that we could only do this 
-because we moved "false" into the context manually when we used
-the "move" tactic. So our math is still consistent and the world hasn't exploded yet.
+because we moved "false" into the context manually when we used the "move" tactic.
+So our math is still consistent and the world hasn't exploded yet.
 The way to think about this triple is assuming "false" holds implies that 15 = 0.
 *)
 
 
-module Flip_Exp = {
+(*
+Let us now work with some more interesting functions and triples.
+The flipper function simply returns the opposite of the boolean
+value that it gets.
+*)
 
-proc flipper (x: bool) : bool =
-{
+module Flip = {
+
+proc flipper (x: bool) : bool = 
+  {
   var r: bool;
   if (x = true) 
   { r <- false; }
   else
   { r <- true; }
   return r;
-}
-
-proc exp (x a: int) : int = 
-{
-  var r;
-  r <- 1;
-  while (a <> 0){
-    r <- r * x;
-    a <- a-1;
   }
-  return r;
-}
-
-
 }.
 
-lemma flipper_correct: hoare [ Flip_Exp.flipper : x = true ==> res = false ].
+lemma flipper_correct: hoare [ Flip.flipper : x = true ==> res = false ].
 proof.
 proc.
 (*
@@ -251,11 +274,11 @@ if.
  
   (* If the current goal is a HL, pHL, pRHL statement the "auto" tactic
     uses various program logic tactics in an attempt to reduce the goal
-    to a simpler one. Never fails, but may fail to make any progress. *)
+    to a simpler one. It never fails, but may fail to make any progress. *)
 
   (* Goal 2: x <> true.
   Yields a contradiction in the assumptions.
-  we can use some automation to deal with it.
+  We will use some automation to deal with it.
   *)
   wp.
   auto.
@@ -265,22 +288,319 @@ qed.
 (*
 Notice the repetition of proof steps in the branches.
 This can be reduced by using tacticals.
-In order to tell EC to repeated use certain tactics on
-resulting goals, we use the ":" tactical.
+In order to tell EC to repeated use certain tactics on all
+resulting goals, we use the ";" tactical.
 So, we can simplify the above proof like so:
 *)
 
-lemma flipper_correct': hoare [ Flip_Exp.flipper : x = false ==> res = true ].
+lemma flipper_correct': hoare [ Flip.flipper : x = false ==> res = true ].
 proof.
 proc.
 if; wp; auto; smt.
 qed.
 
-lemma exp_correct: hoare [ Flip_Exp.exp : x = 10 /\ a = 2 ==> res = 100 ].
+(*
+Let us define the exponentiation function that we saw in the text.
+*)
+
+module Exp = {
+proc exp (x n: int) : int = 
+  {
+  var r, i;
+  r <- 1;
+  i <- 0;
+  while (i < n){
+    r <- r*x;
+    i <- i+1;
+  }
+  return r;
+  }
+}.
+
+
+(*
+Let us formulate a hoare triple that says that exp(10, 2) = 100.
+The triple would be:
+{x = 10 /\ n=2} Flip_Exp.exp {res=100}
+and in EC, we would write it like so.
+*)
+
+lemma ten_to_two: hoare [ Exp.exp : x = 10 /\ n = 2 ==> res = 100 ].
+proof.
+proc.
+
+(*
+When working with tuples EC has the syntax of using backticks (`) to address the tuple.
+So (x,n).`1 refers to x.
+Often the output from EC can be quite hard to read, simplifying it can sometimes help.
+*)
+simplify.
+
+(*
+Now we want to reason with a while loop in the program.
+Thankfully, we can see that the loop only runs twice, since n=2.
+To get a feel of how the program runs we can step through a loop
+using the "unroll" tactic. We need to mention the line number of the
+program where we want the tactic to apply. Like so:
+*)
+unroll 3.
+unroll 4.
+
+(*
+At this point, we now have two if conditions which we know will hold,
+and a while loop for which the condition will not hold. To reason with
+loops and conditions like these EC provides two tactics
+rcondt, and rcondf.
+You can read them as remove condition with a true/false assignment.
+Since here we know that the condition will evaluate to false, we will use the
+rcondf version.
+*)
+
+rcondf 5.
+(*
+Notice how the postcondition now requires the condition for the while loop
+to be false.
+Since it would evaluate to false, EC gets rid of the loop.
+Now we can either use the if tactic that we used earlier to work with the
+if conditions here, but wp is generally strong enough to reason with if conditions.
+So let us make our lives a little easier and use that instead.
+Here, since the program is quite simple, the smt solvers can complete the proof.
+However, pay attention to how hard it gets to read the output
+after the application of wp, and skip.
+*)
+wp.
+skip.
+smt.
+
+(*
+Goal #2:
+Now again, we have two if conditions, that we need to work with.
+The proof proceeds that same as before. wp is strong enough to reason with it.
+*)
+
+wp.
+skip.
+smt.
+qed.
+
+(*
+As usual we could have used some tacticals to shorten the proof.
+So let us do that, to clean up the previous proof.
+*)
+
+lemma ten_to_two_clean: hoare [ Exp.exp : x = 10 /\ n = 2 ==> res = 100 ].
+proof.
+proc.
+unroll 3.
+unroll 4.
+rcondf 5; wp; skip; smt.
+qed.
+
+(*
+For a loop that unrolls twice it is easy to do it manually.
+However, this strategy wouldn't work for a different scenario.
+For instance inorder to prove that the program works correctly we need to prove
+the correctness for every number, so we would prefer to work with abstract symbols
+and not concrete numbers like 10^2.
+In order to work up to it, let us prove that 2^10 works as intended.
+But first, we need to understand that EC was not built for computations.
+It can handle small calculations like we've seen so far but asking EC to do 2^10
+doesn't work as we'd like it to.
+For instance, take a look at the following lemma, and our attempt to prove it.
+*)
+
+lemma twototen: 2^10 = 1024.
+proof.
+trivial.
+simplify.
+auto.
+(*
+None of those tactics do anything 
+Even smt doesn't work.
+You can try it as well.
+Again, the point here is that, these kinds of tasks aren't what EC was
+built for.
+For the time being we will admit this lemma, since we know that
+2^10 is infact 1024.
+We need this to prove the next few lemmas relating to hoare triples.
+*)
+admit.
+qed.
+
+lemma two_to_ten: hoare [ Exp.exp : x = 2 /\ n = 10 ==> res = 1024 ].
 proof.
 proc.
 simplify.
-(* TODO HELP! *)
-while ().
+(* 
+To get rid of the loop, we need understand the behavior of the program, and 
+figure out a loop invariant. This is because we have the tactic:
+"while I"
+Where "I" is the loop invariant, that holds before and after the loop. 
+This essentially means thinking about what the loop actually does,
+and the conditions that hold before and after the execution of the loop.
+We want the invariant to help us prove the goal that we have.
+Which is r = 1024. Let us try to see how we can get there.
+Let us start small and say that we know that (x = 2) holds before
+and after the execution of the loop.
+*)
+while ( x = 2 ).
+(*
+Observe how the goals have changed.
+In Goal #1, the invariant that we propose is in both the pre and post conditions.
+The burden of the proof still lies on us however. Of course, since we don't
+change x, this should hold quite naturally. And we can discharge Goal #1 quite
+easily.
+*)
+wp.
+auto.
 
+(*
+Now let us pay attention to what we have left.
+The second part of the postcondition says 
+forall (i0, r0 : int),
+given that i0 is greater than or equal to n, and x = 2
+then r0 = 1024. 
+That is clearly incorrect, since r0 isn't bound or related to x or i0.
+You are welcome to experiment and try to see how far you can get in
+the proof. However in our attempt, the goal simply becomes harder to read.
+Using wp, and skip introduces memory into the context making it quite difficult to
+read. We will abort this attempt here, and try to think of a stronger invariant.
+*)
+abort.
+
+lemma two_to_ten: hoare [ Exp.exp : x = 2 /\ n = 10 ==> res = 1024 ].
+proof.
+proc.
+
+(*
+As an additional invariant, we know that the loop runs until our
+loop variable i goes from 0, to n. So as an invariant, we have
+0 <= i <= n, and the control exits the loop when ! (i < n).
+Let us try to see what happens if we add this in.
+*)
+while ( x = 2  /\ 0 <= i <= n).
+wp.
+auto.
+smt.
+
+(*
+Let us read what the goal says now.
+Again it says sopmething about r0 without bounding what r0 can be.
+This attempt will also fail.
+So we need to understand what happens to the variable r0, at the end of every
+iteration of the loop.
+*)
+abort.
+
+
+lemma two_to_ten: hoare [ Exp.exp : x = 2 /\ n = 10 ==> res = 1024 ].
+proof.
+proc.
+(*
+We know that after every iteration, the variable r is multiplied by x.
+So in this case, since we have x = 2, essentially at the end of
+i iterations of the loop we have the fact that r = 2^i.
+This is an invariant, and it binds r to the variables that are passed to the
+loop. Let us see if this attempt works.
+*)
+while (x = 2  /\ 0 <= i <= n /\  r = 2^i).
+
+(*
+Again, Goal #1 will go through quite easily.
+*)
+wp.
+skip.
+smt.
+
+(* Goal #2 *)
+wp.
+simplify.
+auto.
+(*
+When the goal is too complicated to read, we can apply the tactic "progress".
+"progress" breaks the goals into simpler ones by repeatedly applying the
+"split", "subst" and "move =>" tactics and trying to solve the trivial goals.
+*)
+progress.
+
+(* 2 ^ 0 = 1 *)
+smt.
+
+(* 2^10 = 1024 *)
+smt.
 qed.
+
+(*
+A point to note here:
+Had we not admitted the lemma twototen the proof would get stuck
+You are welcome to comment it out and try the proof again.
+*)
+
+(*
+So finally, we have an invariant that works.
+Let us clean up the proof, and also if we think about it,
+the condition (x=2) isn't really needed, since the program never
+modifies the value of x. So let us get rid of that condition as well.
+*)
+
+lemma two_to_ten_clean: hoare [ Exp.exp : x = 2 /\ n = 10 ==> res = 1024 ].
+proof.
+proc.
+simplify.
+while ( r = x^i /\ 0 <= i <= n); wp; skip; smt.
+qed.
+
+(*
+Now the proof seems so inocous and straighforward.
+However, it is important to understand that these proofs and
+figuring out the loop invariants always take a few tries, and
+sometimes crafting the right invariant can be an art by itself.
+This also gets quite hard when there are a lot of variables
+to keep track of. So it is good practice to work with smaller examples first.
+*)
+
+
+(*
+Now let us try to work with abstract symbols, the stuff that EC
+was actually built for. Here we mentioned in the text, in order to claim
+that the exp function is correct, we need to have the condition that
+the exponent that we provide is greater than zero.
+We use x0, and n0, inorder to differentiate from the program variables.
+*)
+lemma x0_to_n0_correct x0 n0: 
+  0 <= n0 =>
+  hoare [ Exp.exp : x = x0 /\ n = n0 ==> res = x0 ^ n0 ].
+proof.
+move => Hn0.
+proc.
+while (r=x^i /\ 0 <= i <= n).
+wp.
+skip.
+smt.
+
+wp.
+skip.
+progress.
+smt.
+smt.
+qed.
+
+
+(*
+Again, we can clean up the proof like so:
+*)
+lemma x0_to_n0_correct_clean x0 n0: 
+  0 <= n0 =>
+  hoare [ Exp.exp : x = x0 /\ n = n0 ==> res = x0 ^ n0 ].
+proof.
+move => Hn0.
+proc.
+while (r=x^i /\ 0 <= i <= n); wp; skip; smt.
+qed.
+
+(*
+As an exercise, you can do similar proof for simple mathematical functions.
+For instance
+1. A program to decide the if a given number is even or odd.
+2. A program to compute the factorial of given number. etc.
+*)
